theories/acyclic.v
@@ -4,39 +4,40 @@ From ambig Require Import grammar acyclic_wf.
 
 Section acyclic.
 
-  Context {Σ N : Type} `{Finite N} (G : grammar Σ N).
+  Context {Σ N : Type} `{!EqDecision N} `{!Finite N}.
+  Context (G : grammar Σ N).
 
-  (* On the graph representation of the grammar: direct edge *)
+  Open Scope grammar_scope.
+
+  (* This relation corresponds to directed edges on the graph representation
+     of a grammar. *)
   Inductive succ : relation N :=
     | succ_unary A B φ :
       A ↦ unary B φ ∈ G →
       succ A B
     | succ_left A B E φ :
       A ↦ binary B E φ ∈ G →
-      G ⊨ E ⇒ [] →
+      G ⊨ E => [] →
       succ A B
     | succ_right A B E φ :
       A ↦ binary E B φ ∈ G →
-      G ⊨ E ⇒ [] →
+      G ⊨ E => [] →
       succ A B
     .
 
+  (* The directed edges reversed. *)
   Definition prec : relation N := flip succ.
 
-  (* acyclic grammar *)
-
+  (* A grammar is acyclic if its graph is acyclic, i.e.
+     the `succ` relation is an acyclic relation. *)
   Definition acyclic : Prop := acyclic succ.
 
-  Lemma acyclic_succ_flip_wf :
-    acyclic → wf (flip succ).
-  Proof.
-    intros. eapply acyclic_flip_wf; eauto.
-  Qed.
-
+  (* Both `prec` and `succ` are well-founded for acyclic grammars. *)
+  Lemma acyclic_prec_wf :
+    acyclic → wf prec.
+  Proof. intros. eapply finite_acyclic_flip_wf; eauto. Qed.
   Lemma acyclic_succ_wf :
     acyclic → wf succ.
-  Proof.
-    intros. eapply acyclic_wf; eauto.
-  Qed.
+  Proof. intros. eapply finite_acyclic_wf; eauto. Qed.
 
 End acyclic.
